lean/TestingAeneas/AVLTree_delete.lean
@@ -1,0 +1,679 @@
+import Aeneas
+import TestingAeneas.BSTree
+import TestingAeneas.AVLTree
+import TestingAeneas.Definitions
+
+set_option maxHeartbeats 1000000
+/- set_option maxRecDepth 1000000 -/
+
+open Aeneas Std
+
+section Operations/- {{{ -/
+namespace Spec
+
+def BSTree.rebalance'(tree: BSTree α): BSTree α :=
+  match tree with
+  | Nil => tree
+  | Node value left right =>
+      let bf1 := tree.balancingFactor
+      if bf1 = 2 then
+        match left with
+        | Nil => tree 
+        | Node .. =>
+          let bf2 := left.balancingFactor
+          if bf2 = -1 then
+            /-
+                  X           ⟨X⟩      linux      
+               ⟨Z⟩  ᵈ  >>    Y  ᵈ   >>     Y
+               ᵃ  Y        Z  ᶜ          Z   X
+                 ᵇ ᶜ       ᵃ ᵇ          ᵃ ᵇ ᶜ ᵈ
+            -/
+            
+            Node value left.rotateLeft right |>.rotateRight
+          else 
+            /-
+                   ⟨X⟩
+                  Y  ᵈ  >>     Y
+                Z  ᶜ         Z   X
+               ᵃ ᵇ          ᵃ ᵇ ᶜ ᵈ
+            -/
+            tree.rotateRight
+      else if bf1 = -2 then
+        match right with
+        | Nil => tree
+        | Node .. =>
+          let bf2 := right.balancingFactor
+          if bf2 = 1 then
+            /-
+                 X         ⟨X⟩           
+               ᵃ  ⟨Z⟩  >>  ᵃ  Y    >>     Y
+                 Y  ᵈ       ᵇ  Z        Z   X
+                ᵇ ᶜ           ᶜ ᵈ      ᵃ ᵇ ᶜ ᵈ
+            -/
+            Node value left right.rotateRight |>.rotateLeft
+          else
+            /-
+               ⟨X⟩           
+               ᵃ  Y    >>     Y
+                ᵇ  Z        Z   X
+                  ᶜ ᵈ      ᵃ ᵇ ᶜ ᵈ
+            -/
+            tree.rotateLeft
+      else tree
+
+def BSTree.popLeftmost{α: Type}[LT α][DecidableLT α][Inhabited α]: BSTree α -> BSTree α × α
+| Nil => @panic _ (instInhabitedProd) "Unreachable"
+| Node value Nil right => (right, value)
+| Node value left right => 
+  let (left', popped) := left.popLeftmost
+  let res := Node value left' right
+  (res.rebalance', popped)
+
+def BSTree.delete_rebalance[LT α][DecidableLT α][Inhabited α](value: α): BSTree α -> BSTree α
+| Nil => Nil
+| Node curr left right =>
+  if value < curr then
+    Node curr (left.delete_rebalance value) right |>.rebalance'
+  else if curr < value then
+    Node curr left (right.delete_rebalance value) |>.rebalance'
+  else -- value == curr
+    match left, right with
+    | Nil, right => right
+    | left, Nil => left
+    | left, right => 
+      let (right', leftmost) := right.popLeftmost
+      let res := Node leftmost left right'
+      res.rebalance'
+
+end Spec
+end Operations/- }}} -/
+
+section Lemmas /- {{{ -/
+open testing_aeneas hiding max min BSTree
+attribute [-simp] Bool.exists_bool
+
+namespace Spec
+
+section Rebalance'/- {{{ -/
+
+@[simp] theorem BSTree.rebalance'_toSet[LinearOrder α][IsTotal α (·≤·)](tree: BSTree α)
+: tree.toSet = tree.rebalance'.toSet
+:= by/- {{{ -/
+  cases tree <;> simp [BSTree.rebalance']
+  case Node value left right =>
+    split -- Here there are actually 3 cases
+    case' isTrue => split_ifs <;> cases left -- First case, destructure left
+    case' isFalse => split
+    case' isTrue => split_ifs <;> cases right -- second case, destructure right
+    -- Third case, can be solved through `simp`
+    all_goals simp [BSTree.rotateLeft_toSet, BSTree.rotateRight_toSet]/- }}} -/
+
+
+theorem BSTree.rebalance'.preserves_inv_left{value: Isize}{left right: AVLTree Isize}{bf: I8}
+: let tree := AVLTree.Node value left right bf
+  tree.invariant
+-> tree.toBS.balancingFactor = 2 
+-> left.toBS.balanced -- left.toBS.all_subtrees (·.balancingFactor.natAbs ≤ 1)
+-> right.toBS.balanced -- right.toBS.all_subtrees (·.balancingFactor.natAbs ≤ 1)
+-> ∃ tree' height_decrease,
+    AVLTreeIsize.rebalance_with_height_decrease tree = .ok (tree', height_decrease) ∧
+    tree.toBS.rebalance' = tree'.toBS ∧
+    tree'.invariant ∧ -- TODO: These don't actually depend on AVLTreeIsize, but just on BSTree. Rework them.
+    tree'.toBS.balanced ∧ -- tree'.toBS.all_subtrees (·.balancingFactor.natAbs ≤ 1) ∧
+    (if height_decrease then tree'.toBS.height = tree.toBS.height - 1
+                        else tree'.toBS.height = tree.toBS.height)
+:= by /- {{{ -/
+  sorry
+  /-
+  intro tree tree_inv bf_2 left_bnd right_bnd
+  have ⟨bf_def, left_inv, right_inv⟩ := tree_inv
+  unfold tree at *
+  simp [AVLTreeIsize.rebalance_with_height_decrease.eq_def]
+
+  have: bf = 2#i8 := by -- NOTE: Spiritually this should be just `scalar_tac`.
+    simp only [<-bf_2, bf_def]
+    scalar_tac
+  simp only [AVLTree.toBS] at bf_def
+  simp only [BSTree.rebalance', bf_def]
+  simp [this]
+
+
+  -- The core of the proof relies on the fact that, since we have restricted the values
+  -- that tree.balancingFactor and left.balancingFactor can take, we can actually 
+  -- determine the values of the heights of the relevant subtrees. In particular, we
+  -- can write them as a function of a shared value H.
+  generalize right_H: right.toBS.height = H at *
+  -- We write subtree_H to refer to the proposition that relates subtree's height with H
+  have left_H : left.toBS.height = H + (2: Int) := by 
+    simp [Spec.balancingFactor_Node, this] at tree_inv
+    omega -- scalar_tac doesn't seem to work
+
+  cases left
+  case Nil => 
+    -- Left cannot be nil, because then its balancingFactor would be 0, which we disallow!
+    simp [AVLTreeIsize.balance_factor, Spec.balancingFactor_Node] at bf_2
+    scalar_tac
+  case Node v1 left1 right1 bf1 =>
+    simp at left_inv
+    have ⟨bf1_def, left1_inv, right1_inv⟩ := left_inv
+    simp [bf1_def] at left_bnd
+    simp [AVLTreeIsize.balance_factor, bf1_def]
+
+    -- Depending on the balancing factor of left, we encounter ourselves in the LEFT-LEFT
+    -- or LEFT-RIGHT case. We handle these separately
+    if bf1_is_n1: bf1 = (-1)#i8 then/- {{{ -/
+      simp [bf1_is_n1] at *
+      -- This is the LEFT-RIGHT case, which corresponds to the following shape
+      /-
+               ┌────tree────┐
+               │     H+3    │
+               ▼            ▼
+        ┌────left───┐     right
+        │     H+2   │       H
+        ▼           ▼
+      left1    ┌──right1──┐
+        H      │   H+1    │
+               ▼          ▼
+             left2      right2
+              ≤H          ≤H
+      -/
+      have left1_H: left1.toBS.height = H:= by omega
+      have right1_H: right1.toBS.height = H + 1 := by omega
+      obtain ⟨left1_bnd, right1_bnd⟩ := left_bnd
+
+      -- We can apply the spec of rotateLeft to get to the following
+      -- intermediary step, which is similar to the LEFT-LEFT case.
+      cases right1
+      case Nil =>
+        -- This can't be nil, because otherwise left.balancingFactor could never be negative!
+        simp [bf1_is_n1] at bf1_def
+      case Node v2 left2 right2 bf2 =>
+        simp [BSTree.rotateLeft] at left_H right1_bnd ⊢
+        have: left2.toBS.height ⊔ right2.toBS.height = H := by omega
+        obtain ⟨bf2_bal, left2_bnd, right2_bnd⟩ := right1_bnd
+
+        progress with rotateLeft.spec as ⟨left', left'_spec, left'_inv⟩
+        · simp [*, boundedBalancingFactor_expand (by decide: 1 < 2)]
+        -- After this operation, this is the current state of our tree
+        /-
+                      ┌────tree────┐
+                      │     H+3    │
+                      ▼            ▼
+               ┌───right1──┐     right
+               │   (left') │       H
+               ▼     H+2   ▼
+          ┌───left───┐   right2
+          │ (left1') │  (right1')
+          ▼   H+1    ▼     ≤H
+        left1      left2
+        (left2')   (right2')
+          H          ≤H
+        -/
+        simp only [BSTree.rotateLeft] at left'_spec
+        -- Now we can simply apply the rotateRight spec and solve the goal through simplification
+        progress as ⟨tree', tree'_spec, tree'_inv⟩
+        · simp [*, BSTree.rotateLeft]; omega
+        · simp [*, boundedBalancingFactor_expand (by decide: 1 < 2)]; omega
+        simp [*, BSTree.rotateRight, Nat.max]
+        scalar_tac/- }}} -/
+    else if bf1_is_1: bf1 = 1#i8 then/- {{{ -/
+      simp [bf1_is_1] at *
+      -- We're in the LEFT-LEFT case. This is the general shape of this case
+      /-
+               ┌──tree──┐
+               ▼        ▼
+           ┌─left─┐    right                ┌─────left─────┐
+           ▼      ▼      H                  ▼              ▼
+        ┌left1┐ right1        =======>  ┌─left1─┐      ┌─tree─┐
+        │     │   H                     ▼       ▼      ▼      ▼
+        ▼     ▼                        left2  right2 right1  right
+      left2 right2                      ≤H      ≤H     H       H
+       ≤H     ≤H
+      -/
+      have right1_H: right1.toBS.height = H     := by omega
+      have  left1_H: left1.toBS.height  = H + 1 := by omega
+
+      -- This case can be solved directly by using the rotateRight spec
+      -- However, to do so we need to provide some specific preconditions
+      -- which require manipulating the hypothesis a bit.
+      obtain ⟨left1_bnd, right1_bnd⟩ := left_bnd
+      progress as ⟨tree', tree'_spec,tree'_inv⟩
+      · simp [*]; omega
+      · simp [*, boundedBalancingFactor_expand (by simp : 1 < 2)]
+        omega
+      simp only [BSTree.rotateRight] at tree'_spec
+      simp [*, BSTree.rotateRight, balancingFactor_Node, BSTree.rebalance, Nat.max]
+      split_conj <;> scalar_tac/- }}} -/
+    else/- {{{ -/
+      have bf1_is_0: bf1 = 0#i8 := by scalar_tac
+      simp [bf1_is_0]
+      have right1_H: right1.toBS.height = left1.toBS.height := by simp [bf1_is_0] at bf1_def; omega
+      have  left1_H: left1.toBS.height  = H + 1 := by simp [right1_H] at left_H; omega
+
+      obtain ⟨left1_bnd, right1_bnd⟩ := left_bnd
+      progress as ⟨tree', tree'_spec,tree'_inv⟩
+      · simp [*]; omega
+      · simp [*, boundedBalancingFactor_expand (by simp : 1 < 2)]
+        omega
+      simp [BSTree.rotateRight] at tree'_spec
+      simp [*, BSTree.rotateRight, balancingFactor_Node, BSTree.rebalance, Nat.max]
+      scalar_tac/- }}} -//- }}} -/
+-/
+
+theorem BSTree.rebalance'.preserves_inv_right{value: Isize}{left right: AVLTree Isize}{bf: I8}
+: let tree := AVLTree.Node value left right bf
+  tree.invariant
+-> tree.toBS.balancingFactor = -2
+-> left.toBS.balanced
+-> right.toBS.balanced
+-> ∃ tree' height_decrease,
+    AVLTreeIsize.rebalance_with_height_decrease tree = .ok (tree',height_decrease) ∧
+    tree.toBS.rebalance' = tree'.toBS ∧
+    tree'.invariant ∧
+    tree'.toBS.balanced ∧
+    (if height_decrease then tree'.toBS.height = tree.toBS.height - 1
+                        else tree'.toBS.height = tree.toBS.height)
+:= by /- {{{ -/
+  sorry/-
+  intro tree tree_inv bf_2 left_bnd right_bnd
+  have ⟨bf_def, left_inv, right_inv⟩ := tree_inv
+  unfold tree at *
+  simp [AVLTreeIsize.rebalance_with_height_decrease.eq_def]
+
+  have: bf = (-2)#i8 := by -- NOTE: Spiritually this should be just `scalar_tac`.
+    simp only [<-bf_2, bf_def]
+    scalar_tac
+  simp only [AVLTree.toBS] at bf_def
+  simp only [BSTree.rebalance', bf_def]
+  simp [this]
+
+
+  -- The core of the proof relies on the fact that, since we have restricted the values
+  -- that tree.balancingFactor and left.balancingFactor can take, we can actually 
+  -- determine the values of the heights of the relevant subtrees. In particular, we
+  -- can write them as a function of a shared value H.
+  generalize left_H: left.toBS.height = H at *
+  -- We write subtree_H to refer to the proposition that relates subtree's height with H
+  have right_H : right.toBS.height = H + (2: Int) := by 
+    simp [Spec.balancingFactor_Node, this] at tree_inv
+    omega -- scalar_tac doesn't seem to work
+
+  cases right
+  case Nil => 
+    -- Left cannot be nil, because then its balancingFactor would be 0, which we disallow!
+    simp [AVLTreeIsize.balance_factor, Spec.balancingFactor_Node] at bf_2
+  case Node v1 left1 right1 bf1 =>
+    simp at right_inv
+    have ⟨bf1_def, left1_inv, right1_inv⟩ := right_inv
+    simp [bf1_def] at right_bnd
+    simp [AVLTreeIsize.balance_factor, bf1_def]
+
+    cases bf1_is_1: decide (bf1 = 1#i8)
+    case true =>/- {{{ -/
+      simp at bf1_is_1; simp [bf1_is_1] at *
+
+      have right1_H: right1.toBS.height = H:= by omega
+      have left1_H: left1.toBS.height = H + 1 := by omega
+      obtain ⟨left1_bnd, right1_bnd⟩ := right_bnd
+
+      -- We can apply the spec of rotateLeft to get to the following
+      -- intermediary step, which is similar to the LEFT-LEFT case.
+      cases left1
+      case Nil =>
+        -- This can't be nil, because otherwise left.balancingFactor could never be negative!
+        simp [bf1_is_1] at bf1_def
+        scalar_tac
+      case Node v2 left2 right2 bf2 =>
+        simp [BSTree.rotateRight] at right_H left1_bnd ⊢
+        have: left2.toBS.height ⊔ right2.toBS.height = H := by omega
+        obtain ⟨bf2_bal, left2_bnd, right2_bnd⟩ := left1_bnd
+
+        progress with rotateRight.spec as ⟨right', right'_spec, right'_inv⟩
+        · simp [*, boundedBalancingFactor_expand (by decide: 1 < 2)]
+
+        simp only [BSTree.rotateRight] at right'_spec
+        -- Now we can simply apply the rotateRight spec and solve the goal through simplification
+        progress as ⟨tree', tree'_spec, tree'_inv⟩
+        · simp [*, BSTree.rotateRight]; omega
+        · simp [*, boundedBalancingFactor_expand (by decide: 1 < 2)]; omega
+        simp [*, BSTree.rotateLeft, Nat.max]
+        scalar_tac/- }}} -/
+    cases bf1_is_n1: decide $ bf1 = (-1)#i8
+    case true => /- {{{ -/
+      simp at bf1_is_n1; simp [bf1_is_n1] at *
+      -- We're in the LEFT-LEFT case. This is the general shape of this case
+      /-
+               ┌──tree──┐
+               ▼        ▼
+           ┌─left─┐    right                ┌─────left─────┐
+           ▼      ▼      H                  ▼              ▼
+        ┌left1┐ right1        =======>  ┌─left1─┐      ┌─tree─┐
+        │     │   H                     ▼       ▼      ▼      ▼
+        ▼     ▼                        left2  right2 right1  right
+      left2 right2                      ≤H      ≤H     H       H
+       ≤H     ≤H
+      -/
+      have  left1_H: left1.toBS.height  = H     := by omega
+      have right1_H: right1.toBS.height = H + 1 := by omega
+
+      -- This case can be solved directly by using the rotateRight spec
+      -- However, to do so we need to provide some specific preconditions
+      -- which require manipulating the hypothesis a bit.
+      obtain ⟨left1_bnd, right1_bnd⟩ := right_bnd
+      progress as ⟨tree', tree'_spec,tree'_inv⟩
+      · simp [*]; omega
+      · simp [*, boundedBalancingFactor_expand (by simp : 1 < 2)]
+        omega
+      simp only [BSTree.rotateLeft] at tree'_spec
+      simp [*, BSTree.rotateLeft, balancingFactor_Node, BSTree.rebalance, Nat.max]
+      split_conj <;> scalar_tac/- }}} -/
+    case false =>/- {{{ -/
+      have bf1_is_0: bf1 = 0#i8 := by 
+        simp only [decide_eq_false_iff_not, IScalar.neq_to_neq_val, IScalar.ofInt_val_eq,
+          Int.reduceNeg] at bf1_is_1 bf1_is_n1
+        scalar_tac
+      simp [bf1_is_0]
+      have right1_H: right1.toBS.height = left1.toBS.height := by simp [bf1_is_0] at bf1_def; omega
+      have  left1_H: left1.toBS.height  = H + 1 := by simp [right1_H] at right_H; omega
+
+      obtain ⟨left1_bnd, right1_bnd⟩ := right_bnd
+      progress as ⟨tree', tree'_spec,tree'_inv⟩
+      · simp [*]; omega
+      · simp [*, boundedBalancingFactor_expand (by simp : 1 < 2)]
+        omega
+      simp [BSTree.rotateRight] at tree'_spec
+      simp [*, BSTree.rotateLeft, balancingFactor_Node, BSTree.rebalance, Nat.max]
+      checkpoint scalar_tac/- }}} -//- }}} -/
+-/
+
+theorem BSTree.rebalance'.preserves_wf[LinearOrder α][IsTotal α (·≤·)]{tree: BSTree α}
+: tree.well_formed
+-> tree.rebalance'.well_formed
+:= by/- {{{ -/
+  cases tree 
+  case Nil => simp [BSTree.rebalance']
+  case Node value left right =>
+    simp only [BSTree.rebalance']
+    simp
+    intro left_wf right_wf left_bs right_bs
+    if bf_2: left.height - right.height = (2 : Int) then
+      simp [bf_2]
+      -- In this case, we look at the left
+      cases left
+      case Nil => simp_all
+      case Node v1 left1 right1 =>
+        simp at left_bs ⊢
+        have ⟨left1_wf, right1_wf, left1_bs, right1_bs⟩ := left_wf
+        have v1_value: v1 < value := by apply left_bs; simp
+
+        if bf1_n1: (left1.height - right1.height : Int) = -1 then
+          -- LEFT-RIGHT case
+          simp [bf1_n1]
+
+          cases right1
+          case Nil => 
+            simp [BSTree.rotateRight, BSTree.rotateLeft]
+            split_conjs <;> try assumption
+
+            -- NOTE: Closing dependent arrows{{{
+            intro x x_right
+            trans value <;> try assumption
+            apply right_bs; assumption/- }}} -/
+          case Node v2 left2 right2 =>
+            have ⟨left2_wf, righ2_wf, left2_bs, right2_bs⟩ := right1_wf
+            have v1_v2 : v1 < v2 := by exact right1_bs v2 (by simp)
+            have v2_value : v2 < value := by exact left_bs v2 (by simp)
+
+            simp [BSTree.rotateRight, BSTree.rotateLeft, *]
+
+            -- NOTE: Closing dependent arrows{{{
+            split_conjs <;> try assumption
+            · intro x x_left2; apply right1_bs; simp [*]
+            · intro x x_right2; apply left_bs; simp [*]
+            · intro x h
+              obtain (h | h) | h := h
+              · rw [h]; assumption
+              · trans v1 <;> try assumption
+                apply left1_bs; assumption
+              · apply left2_bs; assumption
+            · intro x h
+              obtain (h | h) | h := h
+              · rw [h]; assumption
+              · apply right2_bs; assumption
+              · trans value <;> try assumption
+                apply right_bs; assumption/- }}} -/
+        else -- if bf1_1: (left1.height - right1.height : Int) = 1 then
+          -- LEFT-LEFT case
+          simp [bf1_n1, BSTree.rotateRight]
+          split_conjs <;> simp_all -- The problem with this simp_all is that it deletes v1_value
+
+          have v1_value: v1 < value := left_bs _ (by simp)
+
+          -- NOTE: Closing dependent arrows{{{
+          intro x hyp 
+          obtain (h | h) | h := hyp
+          · rw [h]; assumption
+          · apply right1_bs; assumption
+          · trans value <;> try assumption
+            apply right_bs; assumption/- }}} -/
+
+    else if bf_n2: (left.height - right.height : Int) = -2 then
+      simp [bf_n2]
+      -- In this case we look at the right.
+      -- It's symmetrical to the previous branch
+      cases right
+      case Nil => simp; split_conjs <;> assumption
+      case Node v1 left1 right1 =>
+        simp at right_bs ⊢
+        have ⟨left1_wf, right1_wf, left1_bs, right1_bs⟩ := right_wf
+        have value_v1: value < v1 := by apply right_bs; simp
+
+        if bf1_n1: (left1.height - right1.height : Int) = 1 then
+          -- RIGHT-LEFT case
+          simp [bf1_n1]
+
+          cases left1
+          case Nil => 
+            simp [BSTree.rotateRight, BSTree.rotateLeft]
+            split_conjs <;> try assumption
+
+            -- NOTE: Closing dependent arrows{{{
+            intro x x_right
+            trans value <;> try assumption
+            apply left_bs; assumption/- }}} -/
+          case Node v2 left2 right2 =>
+            have ⟨left2_wf, righ2_wf, left2_bs, right2_bs⟩ := left1_wf
+            have v1_v2 : v2 <v1  := by exact left1_bs v2 (by simp)
+            have v2_value : value < v2 := by exact right_bs v2 (by simp)
+
+            simp [BSTree.rotateRight, BSTree.rotateLeft, *]
+            -- NOTE: Closing dependent arrows{{{
+            split_conjs <;> try assumption
+            · intro x x_left2; apply right_bs; simp [*]
+            · intro x x_right2; apply left1_bs; simp [*]
+            · intro x h
+              obtain (h | h) | h := h
+              · rw [h]; assumption
+              · trans value <;> try assumption
+                apply left_bs; assumption
+              · apply left2_bs; assumption
+            · intro x h
+              obtain (h | h) | h := h
+              · rw [h]; assumption
+              · apply right2_bs; assumption
+              · trans v1 <;> try assumption
+                apply right1_bs; assumption/- }}} -/
+        else -- if bf1_1: (left1.height - right1.height : Int) = -1 then
+          -- RIGHT-RIGHT case
+          simp [bf1_n1, BSTree.rotateLeft]
+          split_conjs <;> simp_all
+
+          have v1_value: value < v1 := right_bs _ (by simp)
+
+          -- NOTE: Closing dependent arrows{{{
+          intro x hyp
+          obtain (h | h) | h := hyp
+          · rw [h]; assumption
+          · trans value <;> try assumption
+            apply left_bs; assumption
+          · apply left1_bs; assumption/- }}} -/
+    else
+      simp [bf_n2, bf_2]
+      split_conjs <;> assumption/- }}} -/
+
+theorem BSTree.rebalance'.id_if_balanced{value: Isize}{left right: AVLTree Isize}{bf: I8}
+: let tree := AVLTree.Node value left right bf
+  tree.invariant
+→ tree.toBS.balanced
+→ ∃ tree' _hd,
+  AVLTreeIsize.rebalance_with_height_decrease tree = .ok (tree', _hd) ∧
+  tree.toBS.rebalance = tree' ∧
+  tree'.invariant
+:= by/- {{{ -/
+  intro tree ⟨bf_def, left_inv, right_inv⟩ ⟨bf_ne_2, _⟩
+  simp at bf_def
+  rw [AVLTreeIsize.rebalance_with_height_decrease]
+  simp [tree, balancingFactor_Node, bf_def] at bf_ne_2
+  have: ¬ bf.val = 2 := by scalar_tac
+  have: ¬ bf.val = -2 := by scalar_tac
+  simp [BSTree.rebalance, tree, bf_def, *]/- }}} -/
+
+end Rebalance'/- }}} -/
+
+section Delete/- {{{ -/
+
+theorem BSTree.popLeftmost_contains[LinearOrder α][DecidableLT α][Inhabited α]
+{value: α}{tree left right: BSTree α}
+: tree = .Node value left right
+→ let popped := tree.popLeftmost.2
+  popped ∈ tree.toSet
+:= by /- {{{ -/
+  intro popped
+  simp [popped, BSTree.popLeftmost]
+  cases left_def:left
+  case Nil => 
+    simp [popped, BSTree.popLeftmost]
+  case Node value1 left1 right1 =>
+    simp only [BSTree.popLeftmost, ←left_def]
+    left; right
+    apply popLeftmost_contains left_def/- }}} -/
+
+theorem BSTree.delete_of_popLeftmost_of_wf[LinearOrder α][DecidableLT α][Inhabited α]
+{tree: BSTree α}
+: tree.well_formed
+/- → tree.popLeftmost = (tree', popped) -/ 
+→ tree.popLeftmost.1 = tree.delete_rebalance tree.popLeftmost.2
+:= by/- {{{ -/
+  cases tree
+  case Nil => 
+    simp [BSTree.popLeftmost, BSTree.delete_rebalance, panic, panicCore, default]
+  case Node value left right =>
+    cases left_def: left
+    case Nil =>
+      simp [BSTree.popLeftmost, BSTree.delete_rebalance]
+    case Node value1 left1 right1 =>
+      simp only [←left_def]
+      simp [BSTree.popLeftmost, BSTree.delete_rebalance]
+      intro left_wf right_wf left_bs right_bs
+      generalize popped_def: (Spec.BSTree.Node value left right).popLeftmost.2 = popped
+
+      have: popped < value := by
+        apply left_bs popped
+        simp only [left_def, BSTree.popLeftmost] at popped_def
+        simp [←left_def] at popped_def
+        subst popped_def
+        exact popLeftmost_contains left_def
+      simp [this]
+      simp only [left_def, BSTree.popLeftmost] at popped_def ⊢
+      /- obtain ⟨left'_spec, popped_value⟩ := tree'_spec -/
+      simp [←left_def] at popped_def ⊢
+      congr
+      simp [←popped_def]
+      exact delete_of_popLeftmost left_wf/- }}} -/
+
+/- example(s: Set α)(x: α): x ∉ s → s \ {x} = s := by exact? -/
+
+theorem BSTree.delete_rebalance.spec[LinearOrder α][DecidableLT α][Inhabited α]
+{tree: BSTree α}(target: α)
+: tree.is_avl
+→ let tree' := tree.delete_rebalance target
+  tree'.toSet = tree.toSet \ {target} ∧
+  tree'.is_avl
+:= by 
+  intro ⟨tree_bal, tree_wf⟩ tree'
+  cases tree
+  case Nil => simp [tree', BSTree.delete_rebalance]
+  case Node val left right =>
+    obtain ⟨bf_bal,left_bal,right_bal⟩ := tree_bal
+    have ⟨left_wf,right_wf,left_bs,right_bs⟩ := tree_wf
+
+    simp [tree', BSTree.delete_rebalance]
+    cases target_val: compare target val <;> simp [compare_iff] at target_val
+    case eq => 
+      -- We have found the element we want to delete
+      subst target_val; simp
+      cases left_def: left <;> cases right_def: right
+      case Nil.Nil => simp
+      -- We deal with the cases in which we shortcircuit the computation.
+      case Nil.Node val1 left1 right1 |
+           Node.Nil val1 left1 right1 =>
+        simp_all
+        ext x
+        simp_all
+        intro hyp
+        apply ne_of_gt
+        case Nil.Node => exact right_bs x hyp
+        case Node.Nil => exact left_bs x hyp
+      -- Otherwise, we deal with `left` and `right`, ignoring their decomposition.
+      simp only [←left_def, ←right_def]
+      simp [delete_of_popLeftmost_of_wf right_wf]
+      split_conjs
+      · -- NOTE: Reasoning over sets!
+        have ⟨this,_⟩:= delete_rebalance.spec right.popLeftmost.2 ⟨right_bal, right_wf⟩
+        simp [Set.insert_union, this, Set.insert_diff_singleton]
+        rw [Set.union_comm]
+        simp [←Set.insert_union]
+        simp [Set.insert_union]
+        have := BSTree.not_mem_value_of_wf (tree_wf)
+        simp [Set.diff_singleton_eq_self this]
+        simp [←Set.insert_union]
+        simp [Set.insert_eq_self.mpr (popLeftmost_contains right_def)]
+        simp [Set.union_comm]
+      · 
+        sorry
+      · sorry
+    case lt => 
+      simp [target_val]
+      sorry
+    case gt => 
+      simp [target_val]
+      sorry
+
+    obtain target_lt | target_val | target_gt := lt_trichotomy target val
+    · simp [target_lt]
+      
+      sorry
+    · substs target_val
+      simp
+      sorry
+
+    · simp [target_gt, not_lt_of_lt target_gt]
+      sorry
+
+theorem testing_aeneas.AVLTreeIsize.deleteAndWarn.spec
+{tree tree': AVLTree Isize}{target: Isize}
+: tree.invariant
+→ tree.toBS.is_avl
+→ ∃ tree' height_decrease,
+  AVLTreeIsize.deleteAndWarn tree target = Result.ok (tree', height_decrease) ∧
+  tree'.toBS = tree.toBS.delete_rebalance target ∧
+  tree'.invariant ∧
+  if height_decrease then tree'.toBS.height = tree.toBS.height - 1
+                     else tree'.toBS.height = tree.toBS.height
+
+:= by sorry
+
+end Delete/- }}} -/
+
+end Spec
+end Lemmas/- }}} -/
